Add stubs for four key semantic relations
- filtered
- mapped
- grouped
- joined

Relations.v
@@ -16,34 +16,42 @@ with helper(c: col_ty) : Type :=
   end.
 
 
-Inductive relation : schema_ty -> Type :=
-| Relation: forall (s: schema_ty),
-    multiset (support s) -> relation s.
+(* Definition relation : Type := forall s: schema_ty, multiset (support s). *)
 
-(* What's wrong with this way of defining it? *)
-(* Definition relation (s: schema_ty) (rows: list (support s)) : (s, rows). *)
 
-(* TODO: Make equality *)
-Definition relation_eq (s: schema_ty) (r1 r2: relation s) : Prop := (r1 = r2).
+Inductive relation (s: schema_ty) : Type := 
+| Relation: multiset (support s) -> relation s.
 
+
+(*
+Definition relation_schema (r: relation) : schema_ty.
+Proof. inversion r. apply s. Qed.  (* Use proof tactics to extract schema. *)
+
+Definition relation_data (r: relation) : multiset (support (relation_schema r)).
+Proof. inversion r. assert (s = relation_schema r).
+- 
+
+
+Definition relation_has_schema (r: relation) (s: schema_ty) : Prop :=
+  relation_schema r = s.
+
+Definition relation_eq (s: schema_ty) (r1 r2: relation) : Prop :=
+  relation_has_schema r1 s ->
+  relation_has_schema r2 s ->
+  .
+*)
 
 (* An example schema with just one column: a nat column: *)
 Example nat_schema : schema_ty := (CTyNat ***).
-(*
 Example nat_tuple : support nat_schema := 1.
-Example nat_relation : relation nat_schema := relation (Bag (fun (x: nat) => 0)).
-*)
+Example nat_relation : relation nat_schema := Relation nat_schema (EmptyBag nat).
 
 (* An example schema with just one column: a bag (of nat): *)
 Example bag_schema := (CTyBag (CTyNat ***) ***).
-(*
-Example bag_tuple : support bag_schema := [1; 1].
-Example bag_relation : relation bag_schema := [[1; 2]; [1; 2]].
-*)
+Example bag_tuple : support bag_schema := EmptyBag nat.
+Example bag_relation : relation bag_schema := Relation bag_schema (EmptyBag (multiset nat)).
 
 (* An example schema with two cols: nat and bag of nat. *)
 Example nat_bag_schema : schema_ty := CTyNat *** CTyBag (CTyNat ***) ***.
-(*
-Example nat_bag_tuple : support nat_bag_schema := (1, [1; 2; 1]).
-Example nat_bag_relation : relation nat_bag_schema := [(1, [1; 2; 1]); (2, [])].
-*)
+Example nat_bag_tuple : support nat_bag_schema :=  (1, (EmptyBag nat)).
+Example nat_bag_relation : relation nat_bag_schema := Relation nat_bag_schema (EmptyBag (nat * (multiset nat))).
