Base.v
@@ -1,6 +1,10 @@
 Require Export Pig.SfLib.
 Require Export Pig.Schema.
 Require Export Pig.Types.
-Require Export Pig.Joining.
+Require Export Pig.Relations.
+
+Require Export Pig.Filtering.
+Require Export Pig.Mapping.
 Require Export Pig.Grouping.
+Require Export Pig.Joining.
 Require Export Pig.Rearranging.
