Filtering.v
@@ -1,0 +1,10 @@
+Require Export Pig.Relations.
+
+
+Definition filter (s: schema_ty) : Type := (support s) -> bool.
+
+
+Inductive filtered (s: schema_ty): relation s -> filter s -> relation s -> Prop :=
+  | Filtered : forall (f: filter s) (r r': relation s),
+     (* TODO: Add constraints. *)
+     filtered s r f r'.
