Grouping.v
@@ -1,6 +1,22 @@
-Require Export Pig.Schema.
+Require Export Pig.Relations.
+
+
+(* Note: We assume that a GROUP-BY can only be performed using nat columns;
+   it doesn't make sent to group by a bag column. *)
 
 Definition can_group_by (s: schema_ty) (c: col): Prop :=
   schema_column_has_type s c CTyNat.
 
+
+Definition group_schema (s: schema_ty) : schema_ty :=
+  (CTyNat *** (CTyBag s) ***).
+
+
+Inductive grouped (s: schema_ty) : relation s -> col -> relation (group_schema s) -> Prop :=
+| Grouped: forall r c r',
+    (* TODO: Add constraints. *)
+    grouped s r c r'.
+
+
 Definition can_package_by := can_group_by.
+
