Mapping.v
@@ -1,0 +1,8 @@
+Require Export Pig.Relations.
+
+Definition mapper (s s': schema_ty) : Type := (support s) -> (support s').
+
+Inductive mapped (s s': schema_ty) : relation s -> mapper s s' -> relation s' -> Prop :=
+| Mapped: forall (r: relation s) (m: mapper s s') (r': relation s'),
+    (* TODO: Add constraints. *)
+    mapped s s' r m r'.
