Schema.v
@@ -13,11 +13,10 @@ Notation " x '***' y " := (STyPair x y) (at level 51, right associativity).
 
 
 (* Indicates a column within a schema. Used in the JOIN query's BY clauses. *)
-Definition col: Set := nat.
+Definition col := nat.
 
 
 (* Provides evidence that the given column of a given schema has given attr. *)
-
 Inductive schema_column_has_type: schema_ty -> col -> col_ty -> Prop :=
   | SCHAZero: forall (s s': schema_ty) (c: col_ty),
       s = c *** s' ->
@@ -26,48 +25,3 @@ Inductive schema_column_has_type: schema_ty -> col -> col_ty -> Prop :=
       i = S(i') ->
       s = c' *** s' ->
       schema_column_has_type s' i c'.
-
-
-Fixpoint schema_concatenation (s1 s2 : schema_ty): schema_ty :=
-  match s1 with
-  | STyNil => s2
-  | c *** => STyPair c s2
-  | c *** s1' => c *** (schema_concatenation s1' s2)
-  end.
-
-
-Inductive concatenated_schema: schema_ty -> schema_ty -> schema_ty -> Prop :=
-| CatSchemaZeroAttr: forall s,
-    concatenated_schema STyNil s s
-| CatSchemaOneAttr: forall a s,
-    concatenated_schema (a ***) s (a *** s)
-| CatSchemaCons: forall a s1 s2 s3,
-    concatenated_schema s1 s2 s3 ->
-    concatenated_schema (a *** s1) s2 (a *** s3).
-
-
-Lemma schema_concatenation_correct: forall (s1 s2: schema_ty),
-  concatenated_schema s1 s2 (schema_concatenation s1 s2).
-Proof.
-  intros. induction s1.
-  - admit.
-  - admit.
-Admitted.
-
-
-Inductive filter_fn : Set :=
-| FilterFn: id -> schema_ty -> filter_fn.
-
-Inductive map_fn : Set :=
-| MapFn: id -> schema_ty -> map_fn.
-
-
-(* IDEA: Maybe we don't need to model the tuples themselves, just their types.
-         However, we do need to represent sorted lists of tuples, but we can
-         do that using types (see stdlib's `Sorted`). Because of this I am
-         hoping that we don't need to `fuse_tuples`. *)
-
-(*
-Fixpoint fuse_tuples (s1 s2: schema_ty) (t1: support s1) (t2: support s2) :
-                                     support (schema_concatenation s1 s2) := ???
-*)
