Semantics.v
@@ -1,18 +1,4 @@
+Require Export Pig.Schema.
 Require Export Pig.Base.
 
-Section defs.
-
-
-
-(* TODO *)
-(* Provides proof that the output relation is equivalent to the input relation *)
-(*
-Inductive mapped : relation -> relation
-*)
-
-End defs.
-
-  (*
-  Inductive grouped (schema_ty): relation s -> relation -> id :=
-  | t_filter: relation s -> t_filter.
-  *)
+(* TODO: Nothing here yet. *)
